compiler/proof_vec/poly1305_avx_5xp_safe_proof.ec
@@ -2,8 +2,55 @@ require import AllCore List Jasmin_model Int IntDiv CoreMap Poly1305_avx_5xp_saf
 
 hint simplify (oget_some, oget_none).
 
-hoare packS : M.pack : M.safe ==> M.safe.
-proof. by proc; wp; skip; cbv delta. qed.
+op wsize_i (w:wsize) = 
+  with w = W8   => 1
+  with w = W16  => 2
+  with w = W32  => 4
+  with w = W64  => 8
+  with w = W128 => 16
+  with w = W256 => 32.
+
+op is_align : wsize -> W64.t -> bool.
+
+op valid_range (w:wsize) (mem:global_mem_t) (ptr:W64.t) (len:int) =
+  forall i, i < len => is_valid mem (ptr + W64.of_int (wsize_i w * i)) w.
+
+axiom valid_range_size_le w1 w2 mem ptr len : 
+   wsize_i w1 <= wsize_i w2 => 
+   valid_range w2 mem ptr len =>
+   valid_range w1 mem ptr (len * wsize_i w2 %/ wsize_i w1).
+
+axiom valid_range_size_ge w1 w2 mem ptr len1 len2 :
+  is_align w2 ptr => 
+  wsize_i w1 <= wsize_i w2 =>  
+  (wsize_i w2 %/ wsize_i w1) * len2 <= len1 =>
+  valid_range w1 mem ptr len1 =>
+  valid_range w2 mem ptr len2.
+
+lemma ult_of_int x y :
+   (W64.of_int x \ult W64.of_int y) = (x %% W64.modulus < y %% W64.modulus).
+proof. by rewrite W64.wultE /=. qed.
+
+hint simplify ult_of_int.
+
+(* TODO : move this *)  
+lemma is_init_Some4 (t:'a Array4.t) : is_init (map Some t).
+proof. by cbv delta. qed.
+
+lemma is_init_Some5 (t:'a Array5.t) : is_init (map Some t).
+proof. by cbv delta. qed.
+
+hint simplify (is_init_Some4, is_init_Some5)@0.
+
+
+
+hoare packS : M.pack : M.safe /\ valid_range W64 Glob.mem y 2 ==> M.safe.
+proof. 
+  proc; wp; skip => /> &1 _ hv. 
+  have -> : W64.of_int 0 = W64.of_int (8 * 0) by done.
+  have -> : W64.of_int 8 = W64.of_int (8 * 1) by done.
+  by split; apply hv.
+qed.
 
 hoare add_carryS : M.add_carry : M.safe ==> M.safe.
 proof. 
@@ -13,24 +60,27 @@ proof.
   rcondt 44; 1: by auto.
   rcondt 63; 1: by auto.
   rcondf 82; 1: by auto.
-  by wp;skip; cbv delta. 
+  by wp;skip.
 qed.
 
-hoare unpackS : M.unpack : M.safe ==> M.safe.
-proof. by proc; wp; skip; cbv delta. qed.
+hoare unpackS : M.unpack : M.safe /\ valid_range W64 Glob.mem m 2 ==> M.safe.
+proof. 
+  proc; wp; skip; cbv delta => /> &1 _ hv. 
+  have -> : W64.of_int 0 = W64.of_int (8 * 0) by done.
+  have -> : W64.of_int 8 = W64.of_int (8 * 1) by done.
+  by split; apply hv.
+qed.
 
 hoare freezeS : M.freeze : M.safe ==> M.safe.
 proof. 
-  proc; wp. 
-  call add_carryS; wp.
-  by skip; cbv delta.
+  by proc; wp; call add_carryS; wp; skip; cbv delta.
 qed.
 
 hoare carry_reduceS : M.carry_reduce : M.safe ==> M.safe.
-proof. by proc; wp; skip; cbv delta. qed.
+proof. by proc; wp; skip. qed.
 
 hoare mulmod_12S : M.mulmod_12 : M.safe ==> M.safe.
-proof. by proc; wp; skip; cbv delta. qed.
+proof. by proc; wp; skip. qed.
 
 hoare addS : M.add : M.safe ==> M.safe.
 proof. 
@@ -41,44 +91,70 @@ proof.
   rcondt 17; 1: by auto.
   rcondt 22; 1: by auto.
   rcondf 27; 1: by auto.
-  by wp; skip; cbv delta. 
+  by wp; skip.
 qed.
 
-hoare load_lastS : M.load_last : M.safe ==> M.safe.
+(* TODO: move this *)
+lemma nltgeE (x y: W64.t) : (! x \ult y) = (y \ule x).
+proof.
+  rewrite W64.wultE W64.wuleE; smt ().
+qed.
+
+(* TODO: move this *)
+lemma to_uint_minus (x y: W64.t) : y \ule x => to_uint (x - y) = to_uint x - to_uint y.
+proof.
+  rewrite W64.addE W64.oppE /ilift2 /ilift1.
+admitted.
+
+axiom add_of x y : W64.of_int x + W64.of_int y = W64.of_int (x + y).
+axiom addw0 (w:W64.t) : w + W64.of_int 0 = w.
+axiom addwA : associative W64.( + ).
+
+hoare load_lastS : M.load_last : 
+   M.safe /\ valid_range W8 Glob.mem in_0 (W64.to_uint inlen) /\ is_align W64 in_0 ==> M.safe.
 proof. 
-  proc; wp.
+  proc => /=; wp.
   conseq (_: M.safe /\ is_init m). 
   + by cbv delta => />.
-  seq 4: (M.safe /\ is_init m).
-  + rcondt 4; 1: by auto. 
+  seq 4: (#pre /\ is_init m).
+  + conseq />. 
+    rcondt 4; 1: by auto. 
     rcondt 8; 1: by auto.
     rcondf 12; 1: by auto.
     by wp; skip; cbv delta.
   if.
-  + wp; conseq (_ : M.safe /\ is_init n /\ is_init m).
-    + by cbv delta => />.
-    while (M.safe /\ is_init n /\ is_init m /\ is_init c).
-    + wp; skip; cbv delta => />.
+  + wp. 
+    while (M.safe /\ is_init n /\ is_init m /\ is_init c /\ 
+           valid_range W8 Glob.mem in_0 (to_uint inlen)).
+    + wp; skip; cbv delta => /> &1 _ _ _ _ _ hv.
+      move: (odflt _ _) => c1; rewrite W64.wultE => hlt.
+      by rewrite -(W64.to_uintK c1) hv.
     by wp; skip; cbv delta => />.
-  wp; conseq (_ : M.safe /\ is_init n /\ is_init m).
-  + by cbv delta => />.
-  while (M.safe /\ is_init n /\ is_init m /\ is_init c).
-  + wp; skip; cbv delta => />.
-  by wp; skip; cbv delta => />.
+  wp. 
+  while (M.safe /\ is_init n /\ is_init m /\ is_init c /\ 
+         valid_range W8 Glob.mem in_0 (to_uint inlen)).
+  + wp; skip; cbv delta => /> &1 _ _ _ _ _ hv.
+    move: (odflt _ _) => c1; rewrite W64.wultE => hlt.
+    by rewrite -(W64.to_uintK c1) hv.
+  wp; skip; cbv delta => /> &1 _ hv ha _ _.
+  rewrite nltgeE => ^ hule; rewrite W64.wuleE /= => hle.
+  split.
+  + rewrite (_: in_0{1} + W64.of_int 0 = in_0{1}); 1: by ring.
+    have h := (valid_range_size_ge W8 W64 Glob.mem{1} in_0{1} 
+                   (to_uint inlen{1}) 1 ha _ _ hv) => //.
+    by have /= := h 0 _ => //; rewrite addw0.
+  move=> i; rewrite to_uint_minus 1:// (W64.to_uint_small 8) 1:// => h.
+  rewrite -addwA add_of; apply hv => /#.
 qed.
-   
-hoare loadS: M.load : M.safe ==> M.safe.
+  
+hoare loadS: M.load : M.safe /\ valid_range W64 Glob.mem in_0 2 ==> M.safe.
 proof.
-  proc.
-  wp; call unpackS.
-  by wp; skip; cbv delta.  
+  by proc; wp; call unpackS; wp; skip; cbv delta.  
 qed.
 
-hoare clampS : M.clamp : M.safe ==> M.safe.
+hoare clampS : M.clamp : M.safe /\ valid_range W64 Glob.mem k 2 ==> M.safe.
 proof.
-  proc; wp.
-  call unpackS; wp.
-  by skip; cbv delta.  
+  by proc; wp; call unpackS; wp; skip; cbv delta.  
 qed.
 
 hoare unpack_u26x5x2_to_u26x5x2S : M.unpack_u26x5x2_to_u26x5x2 : M.safe ==> M.safe.
@@ -107,10 +183,10 @@ proof.
 qed.
 
 hoare carry_reduce_u128S : M.carry_reduce_u128 : M.safe ==> M.safe.
-proof. by proc; wp; skip; cbv delta => />. qed.
+proof. by proc; wp; skip. qed.
 
 hoare mulmod_u128S : M.mulmod_u128 : M.safe ==> M.safe.
-proof. by proc; wp; skip; cbv delta => />. qed.
+proof. by proc; wp; skip. qed.
 
 hoare add_u128S : M.add_u128 : M.safe ==> M.safe.
 proof. 
@@ -121,21 +197,67 @@ proof.
   rcondt 17; 1: by auto.
   rcondt 22; 1: by auto.
   rcondf 27; 1: by auto.
-  by wp; skip; cbv delta.
+  by wp; skip. 
 qed.
 
-hoare unpack_u128x2_to_u26x5x2S : M.unpack_u128x2_to_u26x5x2 : M.safe ==> M.safe.
-proof. by proc; wp; skip; cbv delta => />. qed.
+hoare unpack_u128x2_to_u26x5x2S : M.unpack_u128x2_to_u26x5x2 : 
+   M.safe /\ valid_range W64 Glob.mem m 4 ==> M.safe.
+proof. 
+  proc; wp; skip; cbv delta => /> &1 _ hv. 
+  rewrite (_: 8 = 8 * 1) 1:// (_: 0 = 8 * 0) 1:// (_: 16 = 8 * 2) 1:// (_: 24 = 8 * 3) 1://.
+  by rewrite !hv.
+qed.
 
 hoare final_mulS : M.final_mul : M.safe ==> M.safe.
 proof.
   proc; wp.
   call hadd_u128S; wp.
   call carry_reduce_u128S; wp.
-  by call mulmod_u128S; wp; skip => />; cbv delta.
+  by call mulmod_u128S; wp; skip.
 qed.
+
+(* TODO: move this *)
+lemma valid_range_add (k:int) w mem ptr len :
+  k <= len =>   
+  valid_range w mem ptr len =>
+  valid_range w mem (ptr + W64.of_int (k * wsize_i w)) (len - k).
+proof.
+  move=> hk hv i hi. 
+  rewrite -addwA add_of. 
+  have -> : k * wsize_i w + wsize_i w * i = wsize_i w * (k + i) by ring.
+  apply hv => /#.
+qed.
+
+(* TODO: move this *)
+lemma valid_range_le (len1 len2:int) w mem ptr  :
+  len1 <= len2 =>   
+  valid_range w mem ptr len2 =>
+  valid_range w mem ptr len1.
+proof. by move=> hle hv i hlt; apply hv => /#. qed.
   
-hoare first_blockS : M.first_block : M.safe ==> M.safe.
+lemma valid_range_add32 mem ptr :
+  valid_range W64 mem ptr 8 =>
+  valid_range W64 mem ptr 4 /\
+  valid_range W64 mem (ptr + W64.of_int 32) 4.
+proof.
+  move=> hv;split.
+  + by apply: valid_range_le hv.
+  by apply (valid_range_add 4 W64 mem ptr 8).
+qed.
+
+lemma valid_range_add16 mem ptr :
+  valid_range W64 mem ptr 4 =>
+  valid_range W64 mem ptr 2 /\
+  valid_range W64 mem (ptr + W64.of_int 16) 2.
+proof.
+  move=> hv;split.
+  + by apply: valid_range_le hv.
+  by apply (valid_range_add 2 W64 mem ptr 4).
+qed.
+
+hoare first_blockS in0 : M.first_block : 
+  M.safe /\ valid_range W64 Glob.mem in_0 8 /\ in_0 = in0 ==>
+  M.safe /\ res.`2 = in0 + W64.of_int 64.
 proof.
   proc; wp.
   call carry_reduce_u128S; wp.
@@ -143,143 +265,236 @@ proof.
   call unpack_u128x2_to_u26x5x2S; wp.
   call mulmod_u128S; wp.
   call unpack_u128x2_to_u26x5x2S; wp.
-  by skip => />; cbv delta.
+  skip => /> &1 _ /valid_range_add32 /> *; ring. 
 qed.
 
-hoare mulmod_add_u128_prefetchS : M.mulmod_add_u128_prefetch : M.safe ==> M.safe.
+hoare mulmod_add_u128_prefetchS : M.mulmod_add_u128_prefetch : 
+  M.safe /\ valid_range W64 Glob.mem in_0 4 ==> M.safe.
 proof.
   proc; wp.
   call unpack_u128x2_to_u26x5x2S; wp.
-  by call add_u128S; wp; skip; cbv delta.
+  by call add_u128S; wp; skip => />; cbv delta.
 qed.
 
-hoare mulmod_u128_prefetchS : M.mulmod_u128_prefetch : M.safe ==> M.safe.
+hoare mulmod_u128_prefetchS : M.mulmod_u128_prefetch : 
+  M.safe /\ valid_range W64 Glob.mem in_0 4 ==> M.safe.
 proof.
   proc; wp.
-  by call unpack_u128x2_to_u26x5x2S; wp; skip; cbv delta.
+  by call unpack_u128x2_to_u26x5x2S; wp; skip => />; cbv delta.
 qed.
 
-hoare remaining_blocksS : M.remaining_blocks : M.safe ==> M.safe.
+hoare remaining_blocksS in0 : M.remaining_blocks : 
+  M.safe /\ valid_range W64 Glob.mem in_0 8 /\ in_0 = in0 ==> 
+  M.safe /\ res.`2 = in0 + W64.of_int 64.
 proof.
   proc; wp.
   call carry_reduce_u128S; wp.
   call add_u128S; wp.
   call mulmod_add_u128_prefetchS; wp.
   call mulmod_u128_prefetchS; wp.
-  by skip; cbv delta.
+  by skip => /> &1 _ /valid_range_add32 /> *; ring.
 qed.
 
-hoare poly1305S : M.poly1305 : M.safe ==> M.safe.
+(* TODO move this *)
+axiom and_mod k w : 
+  0 <= k < W64.size => 
+  to_uint (w `&` W64.of_int (2^k - 1)) = to_uint w %% 2^k.
+
+(* TODO move this *)
+axiom shr_mod (w:W64.t) (i:W8.t) : 
+  to_uint i <= W64.size => to_uint (w `>>` i) = to_uint w %/ 2^ (to_uint i).
+
+(* TODO move this *)
+axiom is_align_add w ptr ofs: 
+  wsize_i w %| W64.to_uint ofs => is_align w ptr => is_align w (ptr + ofs).
+
+lemma to_uint0 : to_uint (W64.of_int 0) = 0.
+proof. by rewrite W64.to_uint_small. qed.
+
+lemma to_uint1 : to_uint (W64.of_int 1) = 1.
+proof. by rewrite W64.to_uint_small. qed.
+
+hint simplify (to_uint0, to_uint1)@0.
+
+axiom to_uint_bounded (w:W64.t) : 0 <= to_uint w < W64.modulus. 
+
+hoare poly1305S : M.poly1305 :
+    M.safe /\
+    valid_range W64 Glob.mem k 4 /\
+    valid_range W8 Glob.mem in_0 (W64.to_uint inlen) /\
+    valid_range W64 Glob.mem out 2 /\
+    is_align W64 in_0
+    ==> 
+    M.safe.
 proof.
-  proc.
-  call packS; wp.
-  call add_carryS; wp.
-  call unpackS; wp.
-  call freezeS; wp.
-  seq 61: (M.safe /\ is_init h /\ is_init s_k /\ is_init s_out); last first.
-  + skip; cbv delta => />.
-  seq 60: (M.safe /\ is_init h /\ is_init s_k /\ is_init s_r /\ is_init s_rx5 /\ is_init s_out); last first.
-  + if => //.
-    wp. 
-    call carry_reduceS; wp.
-    call mulmod_12S; wp.
-    call addS; wp.
-    call load_lastS; wp.
-    by skip; cbv delta => />.
-  wp. 
-  while (M.safe /\ is_init b16 /\ is_init h /\ is_init s_rx5 /\ is_init s_r /\ 
-        is_init s_k /\ is_init s_out /\ is_init s_inlen).
-  + wp.
-    call carry_reduceS; wp.
-    call mulmod_12S; wp.
-    call addS; wp.
-    call loadS; wp.
-    by skip; cbv delta => />.
-  wp.
-  conseq (_: M.safe /\ is_init s_rx5 /\ is_init h /\
-             is_init s_r /\ is_init s_k /\ is_init s_out /\ is_init s_inlen).
-  + by cbv delta => />. 
-  seq 33 : (M.safe /\  is_init s_k /\ is_init s_out /\ is_init s_inlen /\
-               is_init r /\ is_init s_r /\ is_init s_in).
-  + by wp; call clampS; wp; skip; cbv delta.
-  seq 2 : (#pre /\ is_init s_rx5).
-  + rcondt 2; 1: by auto.
-    rcondt 10; 1: by auto.
-    rcondt 18; 1: by auto.
-    rcondt 26; 1: by auto.
-    rcondf 34; 1: by auto.
-    by wp; skip; cbv delta => />.
-  seq 2 : (#pre /\ is_init h).
-  + rcondt 2; 1: by auto.
+  proc => /=.
+  seq 30 : (M.safe /\
+    valid_range W64 Glob.mem (oget s_k + W64.of_int 16) 2 /\
+    valid_range W8 Glob.mem (oget s_in) (W64.to_uint (oget s_inlen)) /\
+    valid_range W64 Glob.mem (oget s_out) 2 /\
+    is_align W64 in_0 /\ 
+    is_init s_out /\ is_init s_in /\ is_init s_inlen /\ is_init s_k /\ is_init r /\ 
+    s_inlen = Some inlen /\ s_in = Some in_0).
+  + by wp; call clampS; wp; skip => /> &hr _ /valid_range_add16 />; cbv delta.
+  seq 5 : (#pre /\ is_init s_r /\ is_init s_rx5).
+  + conseq />. 
+    rcondt 5; 1: by auto.
+    rcondt 13; 1: by auto.
+    rcondt 21; 1: by auto.
+    rcondt 29; 1: by auto.
+    rcondf 37; 1: by auto.
+    by wp; skip; cbv delta.
+  seq 8 : (#pre /\ is_init h /\ is_init b64 /\ to_uint (oget b64) = to_uint inlen %/ 64).
+  + conseq />.
+    rcondt 2; 1: by auto.
     rcondt 6; 1: by auto.
     rcondt 10; 1: by auto.
     rcondt 14; 1: by auto.
     rcondt 18; 1: by auto.
     rcondf 22; 1: by auto.
-    by wp; skip; cbv delta => />.
-  seq 6 : (#pre /\ is_init b64).
-  + by wp; skip; cbv delta.
-  if => //.
-  seq 15 : (#pre /\ is_init s_b64 /\ is_init r2 /\ is_init s_r2 /\ b64 = s_b64).
-  + wp. 
-    call carry_reduceS; wp. 
-    call mulmod_12S; wp.
-    by skip; cbv delta => />  &1; case (b64{1}); cbv delta. 
-  seq 2 : (#pre /\ is_init s_r2x5).
-  + rcondt 2; 1: by auto.
-    rcondt 10; 1: by auto.
-    rcondt 18; 1: by auto.
-    rcondt 26; 1: by auto.
-    rcondf 34; 1: by auto.
-    by wp; skip; cbv delta => />.
-  seq 9 : (#pre /\ is_init r2r /\ is_init s_r2r).
-  + by wp; call unpack_u26x5x2_to_u26x5x2S; wp; skip; cbv delta => />.
-  seq 2 : (#pre /\ is_init s_r2rx5).
-  + rcondt 2; 1: by auto.
-    rcondt 10; 1: by auto.
-    rcondt 18; 1: by auto.
-    rcondt 26; 1: by auto.
-    rcondf 34; 1: by auto.
-    by wp; skip; cbv delta => />.
-  seq 6 : (#pre /\ is_init r2r2 /\ is_init s_r2r2).
-  + wp; call unpack_u26x5x2_to_u26x5x2S; wp.
-    by skip; cbv delta => />.  
-  seq 2 : (#pre /\ is_init s_r2r2x5).  
-  + rcondt 2; 1: by auto.
-    rcondt 10; 1: by auto.
-    rcondt 18; 1: by auto.
-    rcondt 26; 1: by auto.
-    rcondf 34; 1: by auto.
-    by wp; skip; cbv delta => />.
-  seq 4 : (#pre).
-  + by wp; skip => /> => &1; case (s_b64{1}); cbv delta. 
-  seq 1 : (#pre /\ (W64.of_uint 1 \ult oget b64 => 
-                     is_init r4 /\ is_init r4r4 /\ is_init s_r4r4 /\ is_init s_r4r4x5)).
-  + if => //.
-    seq 15 : (#pre /\ is_init r4 /\ is_init r4r4 /\ is_init s_r4r4).
-    + wp. call unpack_u26x5x2_to_u26x5x2S; wp.
-      call carry_reduceS; wp.
-      call mulmod_12S; wp.
-      by skip => />; cbv delta => />.
-    rcondt 2; 1: by auto.
-    rcondt 10; 1: by auto.
-    rcondt 18; 1: by auto.
-    rcondt 26; 1: by auto.
-    rcondf 34; 1: by auto.
-    by wp; skip => />; cbv delta => />.
-  wp; call final_mulS; wp.
-  seq 7 : (#pre /\ is_init hxy).
-  + by wp; call first_blockS; wp; skip => />; cbv delta.
-  case : ((of_uint 1)%W64 \ult oget b64).
-  + while (M.safe /\ is_init s_b64 /\ is_init b64 /\
-            is_init s_r2r2x5 /\ is_init s_r2r2 /\ 
-            is_init s_r4r4x5 /\ is_init s_r4r4 /\ is_init hxy).
-    + by wp; call remaining_blocksS; wp; skip; cbv delta => />.
-    wp; skip => />; cbv delta => /#.
-  rcondf 8.
+    wp; skip => /> &1.
+    by rewrite (shr_mod inlen{1} (W8.of_int 6)) //=; cbv delta.
+  seq 1 : (M.safe /\
+           valid_range W64 Glob.mem (oget s_k + (of_int 16)%W64) 2 /\
+           valid_range W8 Glob.mem in_0 (to_uint (oget s_inlen) %% 64) /\
+           valid_range W64 Glob.mem (oget s_out) 2 /\
+           is_align W64 in_0 /\ is_init s_out /\ is_init s_in /\ is_init s_inlen /\ 
+           is_init s_k /\ is_init s_r /\ is_init s_rx5 /\ is_init h).
+  + if; last first.
+    + skip => /> &1 ?? hv ?????????????.
+      apply: valid_range_le hv.  
+      by rewrite {2} (divz_eq (to_uint inlen{1}) 64); smt (divz_ge0 to_uint_bounded).
+    seq 17 : (#pre /\ is_init s_b64 /\ is_init r2 /\ is_init s_r2 /\ is_init s_r2x5 /\
+              oget s_b64 = oget b64).
+    + conseq />.
+      rcondt 17; 1:by auto.
+      rcondt 25; 1:by auto.
+      rcondt 33; 1:by auto.
+      rcondt 41; 1:by auto.
+      rcondf 49; 1:by auto.
+      wp; call carry_reduceS.
+      wp; call mulmod_12S.
+      by wp; skip => />; cbv delta.
+    seq 11 : (#pre /\ is_init s_r2r /\ is_init s_r2rx5).
+    + conseq />.
+      rcondt 11; 1:by auto.
+      rcondt 19; 1:by auto.
+      rcondt 27; 1:by auto.
+      rcondt 35; 1:by auto.
+      rcondf 43; 1:by auto.
+      by wp; call unpack_u26x5x2_to_u26x5x2S; wp; skip => />; cbv delta.
+    seq 8 : (#pre /\ is_init s_r2r2 /\ is_init s_r2r2x5).
+    + conseq />.    
+      rcondt 8; 1:by auto.
+      rcondt 16; 1:by auto.
+      rcondt 24; 1:by auto.
+      rcondt 32; 1:by auto.
+      rcondf 40; 1:by auto.
+      by wp; call unpack_u26x5x2_to_u26x5x2S; wp; skip => />; cbv delta.
+    seq 4 : (#pre).
+    + by wp; skip => /> &1 ???????????????????? ->.
+    seq 1 : (#pre /\ 
+         (W64.of_int 1 \ult oget b64 => (is_init s_r4r4 /\ is_init s_r4r4x5))).
+    + conseq />; if => //.
+      rcondt 17; 1:by auto.
+      rcondt 25; 1:by auto.
+      rcondt 33; 1:by auto.
+      rcondt 41; 1:by auto.
+      rcondf 49; 1:by auto.
+      wp; call unpack_u26x5x2_to_u26x5x2S.
+      wp; call carry_reduceS.
+      by wp; call mulmod_12S; wp; skip => />; cbv delta.
+    wp; call final_mulS; wp.
+    conseq (_: M.safe /\ is_align W64 in_0 /\ is_init hxy /\
+               valid_range W8 Glob.mem in_0 (to_uint (oget s_inlen) %% 64)) => //.
+    while (M.safe /\ is_align W64 in_0 /\ 
+           is_init b64 /\
+           is_init s_r2r2 /\ is_init s_r2r2x5 /\ is_init hxy /\
+           (W64.of_int 0 \ult oget b64 => is_init s_r4r4x5 /\ is_init s_r4r4) /\
+           valid_range W8 Glob.mem in_0 (to_uint (oget b64) * 64 + to_uint (oget s_inlen) %% 64)).
+    + wp. exists * in_0; elim * => in0.
+      call (remaining_blocksS in0); wp; skip => /> &hr _ ha ???? h hv ^ /h /> ??.
+      rewrite !W64.wultE /= => ?;split.
+      + apply: valid_range_size_ge hv=> //=. 
+        by rewrite (_:8 %/ 1 * 8 = 64) 1://; smt (modz_ge0).
+      move=> ????? ->; rewrite is_align_add //=.
+      have := valid_range_add 64 _ _ _ _ _ hv; 1:smt (modz_ge0).
+      rewrite to_uint_minus 1:W64.wuleE /= /#. 
+    wp. exists * (oget s_in); elim * => in0.      
+    call (first_blockS in0); wp; skip => /> &1 _ ? hv ??????????? hd.
+    rewrite !W64.wultE /= => h0gt ???? -> ???? h1.
+    move:hv; have := divz_eq (to_uint inlen{1}) 64.
+    rewrite -hd => {1}-> hv;split.
+    + apply: valid_range_size_ge hv => //=.
+      by rewrite (_:8 %/ 1 * 8 = 64) 1://; smt (modz_ge0).
+    move=> ???? -> />;split.
+    + rewrite to_uint_minus 1:W64.wuleE /= 1:/# is_align_add //=.
+      split; 1: smt().
+      by have := valid_range_add 64 _ _ _ _ _ hv; smt (modz_ge0).
+    move=> ????; rewrite nltgeE W64.wuleE /=.
+    smt (to_uint_bounded).
+      
+  seq 16 : (M.safe /\
+           valid_range W64 Glob.mem (oget s_k + (of_int 16)%W64) 2 /\
+           valid_range W8 Glob.mem in_0 (to_uint inlen) /\
+           valid_range W64 Glob.mem (oget s_out) 2 /\ is_align W64 in_0 /\
+           is_init s_out /\ is_init s_in /\ is_init s_inlen /\ 
+           is_init s_k /\ is_init s_r /\ is_init s_rx5 /\ is_init h).
   + wp.
-    conseq (_:true) => //.  
-    move => &1 /> _ _ _ _ _ _ _ _ _ _ h1 _ _ _ _ _ _ _ _ _ _ _ _ h2.
-    admit. (* stuff on comparison *)
-  by wp; skip => />; cbv delta.
+    while (M.safe /\
+           valid_range W8 Glob.mem in_0 
+              (to_uint (oget b16) * 16 + to_uint (oget s_inlen) %% 16) /\
+           is_align W64 in_0 /\ is_init s_r /\ is_init s_rx5 /\ is_init h /\ is_init b16). 
+    + wp; call carry_reduceS.
+      wp; call mulmod_12S.
+      wp; call addS.
+      wp; call loadS; wp; skip => /> &1 _ hv ha _ _ _ _.
+      rewrite W64.wultE /= => ?;split.
+      + apply: valid_range_size_ge hv => //.
+        have ->: wsize_i W64 %/ wsize_i W8 = 8 by done.
+        smt (modz_ge0).
+      move=> _; rewrite is_align_add 1://= 1://.
+      have := valid_range_add 16 W8 _ _ _ _ hv; 1: smt (modz_ge0).
+      rewrite (_: 16 * wsize_i W8 = 16) 1://.
+      have -> />: 
+        to_uint (oget b16{1} - (of_int 1)%W64) * 16 + to_uint (oget s_inlen{1}) %% 16 = 
+        to_uint (oget b16{1}) * 16 + to_uint (oget s_inlen{1}) %% 16 - 16.
+      rewrite to_uint_minus; 2: by ring. 
+      by rewrite W64.wuleE /= /#.
+    wp; skip => /> &hr _ _ hv _ ha _ _ _ _ _ _ _;split.
+    + have heq : forall x, x %/ 16 %% 4 = x %% 64 %/ 16.
+      + move=> x; rewrite {1} (divz_eq x 64) {1}(divz_eq (x%%64) 16).
+        rewrite addzA divzDl.
+        + by apply dvdzD; apply dvdz_mull.
+        rewrite (divz_small (x %% 64 %% 16) 16).
+        + by have []:= edivzP (x %% 64) 16.
+        rewrite addz0 divzDr; 1: by apply dvdz_mull.
+        rewrite mulzK 1:// {2}(_:64 = 4 * 16) 1:// -mulzA mulzK 1:// modzMDl.
+        rewrite modz_small 2://;split.
+        + by rewrite divz_ge0 1:// modz_ge0.
+        by move=> _;rewrite ltz_divLR //; apply ltz_pmod.
+      have := and_mod 2 (oget s_inlen{hr} `>>` (of_int 4)%W8) _; 1:by done.
+      rewrite (_: 2^2-1 = 3) 1:// /= => ->.
+      rewrite shr_mod 1:// (_ : 2 ^ to_uint ((W8.of_int 4)) = 16) 1:// heq.  
+      have <- := modz_dvd (to_uint (oget s_inlen{hr})) 64 16 _; 1: done.
+      by rewrite -divz_eq hv.   
+    have /= -> := and_mod 4 (oget s_inlen{hr}) _; 1: done.
+    move=> ? b16 ? ?; rewrite nltgeE W64.wuleE /= => ? _ h1 _ _ _.
+    apply: valid_range_le h1; smt (to_uint_bounded).
+
+  call packS; wp. 
+  call add_carryS; wp.
+  call unpackS; wp. 
+  call freezeS; wp.
+  conseq (_: M.safe /\ 
+             valid_range W64 Glob.mem (oget s_k + (of_int 16)%W64) 2 /\
+             valid_range W64 Glob.mem (oget s_out) 2 /\
+             is_init h /\ is_init s_k /\ is_init s_out).
+  + by move=> />; cbv delta.
+  if => //.
+  wp; call carry_reduceS.
+  wp; call mulmod_12S.
+  wp; call addS.
+  by wp; call load_lastS; skip. 
 qed.
+
